src/Util/ListUtil/RemoveN.v
@@ -5,11 +5,11 @@ Local Open Scope list_scope.
 Module List.
   Section __.
     Context {A} (f : A -> bool).
-    Fixpoint filtern (l : list A) (n : nat) : list A
+    Fixpoint removen (l : list A) (n : nat) : list A
       := match n, l with
          | O, _ => l
          | _, [] => []
-         | S n', x :: xs => if f x then filtern xs n' else x :: filtern xs n
+         | S n', x :: xs => if f x then removen xs n' else x :: removen xs n
          end.
   End __.
 End List.
